amelioration

ILLVarInt.v
@@ -160,7 +160,7 @@ Module M.
   Definition appears_in_env v := exists_in_env (appears true v).
 
   Lemma iter_bool_proper : forall v, Morphisms.Proper
-    (ILLVarInt.MILL.eq ==> Logic.eq ==> Logic.eq ==> Logic.eq)
+    (MILL.eq ==> Logic.eq ==> Logic.eq ==> Logic.eq)
     (iter bool
       (λ (k0 : formula) (acc : bool), (appears true v k0 || acc)%bool)).
   Proof.
@@ -633,6 +633,1787 @@ Module M.
     apply not_exists_in_env_in with (Γ:=Γ\!p); assumption.
   Qed.  
 
+
+Function sub_formula (φ ψ:formula) {struct ψ} : bool := 
+  if FormulaOrdered.eq_dec φ ψ 
+    then true 
+    else
+      match ψ with 
+        | Implies f1 f2 | Otimes f1 f2 | Oplus f1 f2 | And f1 f2 =>
+          orb (sub_formula φ f1) (sub_formula φ f2)
+        | Bang f => sub_formula φ f
+        | _ => false
+      end
+      .
+
+
+Function contains_arrow (φ:formula) {struct φ} : bool := 
+  match φ with 
+    | Implies f1 f2 => true
+    | Otimes f1 f2 | Oplus f1 f2 | And f1 f2 =>
+      orb (contains_arrow f1) (contains_arrow f2)
+    | Bang f => contains_arrow f
+    | _ => false
+  end.
+
+
+Function is_arrows_of_prop (φ:formula) {struct φ} : bool := 
+  match φ with 
+    | Proposition _ => true 
+    | Implies (Proposition _) f2 => is_arrows_of_prop f2
+    | _ => false
+  end.
+
+Function arrow_from_prop (φ:formula) {struct φ} : bool := 
+  match φ with 
+    | Implies _ _  => is_arrows_of_prop φ
+    | Otimes f1 f2 | Oplus f1 f2 | And f1 f2 =>
+      andb (arrow_from_prop f1) (arrow_from_prop f2)
+    | Bang f => arrow_from_prop f
+    | Proposition _ => true 
+    | _ => true
+  end.
+
+Lemma is_arrows_of_prop_arrow_from_prop : 
+  ∀ (φ:formula), is_arrows_of_prop φ = true -> arrow_from_prop φ = true.
+Proof.
+  intros φ.
+  functional induction (is_arrows_of_prop φ).
+  reflexivity.
+  simpl;tauto.
+  discriminate.
+Qed.
+
+Set Implicit Arguments.
+
+
+Lemma proof_of_var : forall Γ ψ, Γ⊢ψ -> forall n, ψ =  Proposition n ->
+  (∀ φ', φ'∈Γ -> sub_formula Zero φ' = false) ->
+  exists φ, φ∈Γ/\ sub_formula (Proposition n) φ = true.
+Proof.
+  intros Γ ψ H.
+  induction H;intros n Heq Hnotzero;try discriminate.
+
+  Focus.
+  subst.
+  exists (Proposition n);split.
+  rewrite H.
+  apply add_is_mem.
+  apply FormulaOrdered.eq_refl.
+  simpl.
+  case (FormulaOrdered.eq_dec (Proposition n) (Proposition n)).
+  reflexivity.
+  intros abs.
+  elim abs;apply FormulaOrdered.eq_refl.  
+
+  Focus.
+  subst.
+  destruct (IHILL_proof2 n (refl_equal _)) as [φ [h1 h2]].
+  intros φ' H3.
+  destruct (mem_destruct _ _ _ H3);clear H3.
+  apply eq_is_eq in H4;subst.
+  generalize (Hnotzero _ H).
+  simpl.
+  intros h;rewrite Bool.orb_false_iff in h;destruct h;assumption.
+  apply Hnotzero.
+  apply mem_remove_2 with (b:=p ⊸ q).
+  rewrite H0;apply mem_union_r;assumption.
+  destruct (mem_destruct _ _ _ h1);clear h1.
+  apply eq_is_eq in H3;subst.
+  exists (p ⊸ q);split.
+  assumption.
+  simpl;rewrite h2;  apply Bool.orb_true_r.
+  exists φ;split;try assumption.
+  apply mem_remove_2 with (b:=p ⊸ q).
+  rewrite H0;apply mem_union_r;assumption.
+
+  Focus.
+  subst.
+  destruct (IHILL_proof _ (refl_equal _)).
+  intros φ' H1.
+  assert (H2 := Hnotzero _ H);simpl in H2.
+  rewrite Bool.orb_false_iff in H2;destruct H2.
+  destruct (mem_destruct _ _ _ H1) as [H4|H4];clear H1.
+  apply eq_is_eq in H4;subst;assumption.
+  destruct (mem_destruct _ _ _ H4) as [H1|H1];clear H4.
+  apply eq_is_eq in H1;subst;assumption.
+  apply Hnotzero.
+  eauto using mem_remove_2.
+  destruct H1 as [H1 H2].
+  destruct (mem_destruct _ _ _ H1) as [H4|H4];clear H1.
+  apply eq_is_eq in H4;subst.
+  exists (p⊗q);split;try assumption.
+  simpl;rewrite H2;auto with bool.
+  destruct (mem_destruct _ _ _ H4) as [H1|H1];clear H4.
+  apply eq_is_eq in H1;subst.
+  exists (p⊗q);split;try assumption.
+  simpl;rewrite H2;auto with bool.
+  exists x;split.
+  eauto using mem_remove_2.
+  assumption.
+
+  Focus.
+  subst.
+  destruct (IHILL_proof _ (refl_equal _)).
+  intros φ' H1.
+  eauto using mem_remove_2.
+  destruct H1 as [H1 H2].
+  exists x;split.
+  eauto using mem_remove_2.
+  assumption.
+
+  Focus.
+  subst.
+  destruct (IHILL_proof _ (refl_equal _)).
+  intros φ' H1.
+  assert (H2 := Hnotzero _ H);simpl in H2.
+  rewrite Bool.orb_false_iff in H2;destruct H2.
+  destruct (mem_destruct _ _ _ H1) as [H4|H4];clear H1.
+  apply eq_is_eq in H4;subst;assumption.
+  apply Hnotzero.
+  eauto using mem_remove_2.
+  destruct H1 as [H1 H2].
+  destruct (mem_destruct _ _ _ H1) as [H4|H4];clear H1.
+  apply eq_is_eq in H4;subst.
+  exists (p&q);split;try assumption.
+  simpl;rewrite H2;auto with bool.
+  exists x;split.
+  eauto using mem_remove_2.
+  assumption.
+
+  Focus.
+  subst.
+  destruct (IHILL_proof _ (refl_equal _)).
+  intros φ' H1.
+  assert (H2 := Hnotzero _ H);simpl in H2.
+  rewrite Bool.orb_false_iff in H2;destruct H2.
+  destruct (mem_destruct _ _ _ H1) as [H4|H4];clear H1.
+  apply eq_is_eq in H4;subst;assumption.
+  apply Hnotzero.
+  eauto using mem_remove_2.
+  destruct H1 as [H1 H2].
+  destruct (mem_destruct _ _ _ H1) as [H4|H4];clear H1.
+  apply eq_is_eq in H4;subst.
+  exists (p&q);split;try assumption.
+  simpl;rewrite H2;auto with bool.
+  exists x;split.
+  eauto using mem_remove_2.
+  assumption.
+
+  Focus.
+  subst.  
+  clear H1.
+  destruct (IHILL_proof1 _ (refl_equal _)).
+  intros φ' H1.
+  assert (H2 := Hnotzero _ H);simpl in H2.
+  rewrite Bool.orb_false_iff in H2;destruct H2.
+  destruct (mem_destruct _ _ _ H1) as [H4|H4];clear H1.
+  apply eq_is_eq in H4;subst;assumption.
+  apply Hnotzero.
+  eauto using mem_remove_2.
+  destruct H1 as [H1 H2].
+  destruct (mem_destruct _ _ _ H1) as [H4|H4];clear H1.
+  apply eq_is_eq in H4;subst.
+  exists (p⊕q);split;try assumption.
+  simpl;rewrite H2;auto with bool.
+  exists x;split.
+  eauto using mem_remove_2.
+  assumption.
+
+  Focus.
+  assert (H1:=Hnotzero _ H);simpl in H1;discriminate.
+
+  Focus.
+  subst.  
+  destruct (IHILL_proof _ (refl_equal _)).
+  intros φ' H1.
+  assert (H2 := Hnotzero _ H);simpl in H2.
+  destruct (mem_destruct _ _ _ H1) as [H4|H4];clear H1.
+  apply eq_is_eq in H4;subst;assumption.
+  apply Hnotzero.
+  eauto using mem_remove_2.
+  destruct H1 as [H1 H2].
+  destruct (mem_destruct _ _ _ H1) as [H4|H4];clear H1.
+  apply eq_is_eq in H4;subst.
+  exists (!p);split;try assumption.
+  exists x;split.
+  eauto using mem_remove_2.
+  assumption.
+
+  Focus.
+  subst.  
+  destruct (IHILL_proof _ (refl_equal _)).
+  intros φ' H1.
+  assert (H2 := Hnotzero _ H);simpl in H2.
+  destruct (mem_destruct _ _ _ H1) as [H4|H4];clear H1.
+  apply eq_is_eq in H4;subst;assumption.
+  apply Hnotzero.
+  eauto using mem_remove_2.
+  destruct H1 as [H1 H2].
+  destruct (mem_destruct _ _ _ H1) as [H4|H4];clear H1.
+  apply eq_is_eq in H4;subst.
+  exists (!p);split;try assumption.
+  exists x;split.
+  eauto using mem_remove_2.
+  assumption.
+
+  Focus.
+  subst.  
+  destruct (IHILL_proof _ (refl_equal _)).
+  intros φ' H1.
+  assert (H2 := Hnotzero _ H);simpl in H2.
+  eauto using mem_remove_2.
+  destruct H1 as [H1 H2].
+  exists x;split.
+  eauto using mem_remove_2.
+  assumption.
+Qed.
+
+Lemma unusable_implies_aux: 
+  ∀ n Γ ψ (p:Γ⊢ψ) φ (Hin:((Proposition n) ⊸φ) ∈ Γ) 
+  (Htopr:sub_formula (⊤) ψ = false)  (Harrr:contains_arrow ψ = false)
+  (Harr:(∀ φ', φ' ∈ Γ -> contains_arrow φ' = true -> arrow_from_prop φ' = true))
+  (Hzero:(∀ φ', φ'∈Γ -> sub_formula Zero φ' = false))
+  (Htop:(∀ φ', φ'∈Γ -> sub_formula (⊤) φ' = false))
+  (Hsub:(∀ φ', φ'∈Γ -> sub_formula (Proposition n) φ' = true  -> ((Proposition n)⊸φ) = φ')),
+  False.
+Proof.
+  induction 1;intros.
+
+  Focus.
+  assert (Htop':= Htop _ Hin).
+  simpl in Htop'.
+  rewrite H in Hin.
+  destruct (mem_destruct _ _ _ Hin);clear Hin.
+  apply eq_is_eq in H0;subst.
+  simpl in *.
+  discriminate.
+  rewrite empty_no_mem in H0;discriminate.
+
+  Focus.
+  discriminate.
+
+  Focus.
+  case (FormulaOrdered.eq_dec ((Proposition n) ⊸ φ) (p1⊸q));intros Heq.
+  (* Top application *)
+  apply eq_is_eq in Heq;injection Heq;clear Heq;intros;subst.
+  assert (proof_of_var' := @proof_of_var _ _ p2 _ (refl_equal _)).
+  destruct (proof_of_var') as [φ' [h1 h2]].
+  intros φ' H6.
+  apply Hzero.
+  apply mem_remove_2 with (Proposition n ⊸ q);rewrite H0;apply mem_union_l; assumption.
+  apply Hsub in h2.
+  2:apply mem_remove_2 with (Proposition n ⊸ q);rewrite H0;apply mem_union_l; assumption.
+  subst.
+  apply IHp1 with (φ:=q);try assumption.
+  simpl;tauto.
+  simpl;tauto.
+  intros φ' H1 H2.
+  apply Harr;try assumption.
+  apply mem_remove_2 with (Proposition n ⊸ q);rewrite H0;apply mem_union_l; assumption.
+  intros φ' H1.
+  apply Hzero;try assumption.
+  apply mem_remove_2 with (Proposition n ⊸ q);rewrite H0;apply mem_union_l; assumption.
+  intros φ' H1.
+  apply Htop;try assumption.
+  apply mem_remove_2 with (Proposition n ⊸ q);rewrite H0;apply mem_union_l; assumption.
+  intros φ' H1 H2.
+  apply Hsub;try assumption.
+  apply mem_remove_2 with (Proposition n ⊸ q);rewrite H0;apply mem_union_l; assumption.
+  (* not top application *)
+  assert (Hin':(Proposition n ⊸ φ)∈(Δ∪Δ')).
+  rewrite <- H0.
+  rewrite <- mem_remove_1.
+  exact Hin.
+  assumption.
+  destruct (mem_union_destruct _ _ _ Hin') as [Hin1|Hin1].
+  (* in Δ *)
+  apply (IHp1 _ Hin1);try assumption.
+  assert (Htop' := Htop _ H).
+  simpl in Htop';rewrite Bool.orb_false_iff in Htop';destruct Htop';assumption.
+  assert (Harr' := Harr _ H (refl_equal _)).
+  simpl in Harr'. 
+  destruct p1;try discriminate.
+  simpl;reflexivity.
+  intros φ' H1 H2.
+  apply Harr;try assumption.
+  apply mem_remove_2 with (p1 ⊸ q);rewrite H0;apply mem_union_l; assumption.
+  intros φ' H1.
+  apply Hzero;try assumption.
+  apply mem_remove_2 with (p1 ⊸ q);rewrite H0;apply mem_union_l; assumption.
+  intros φ' H1.
+  apply Htop;try assumption.
+  apply mem_remove_2 with (p1 ⊸ q);rewrite H0;apply mem_union_l; assumption.
+  intros φ' H1 H2.
+  apply Hsub;try assumption.
+  apply mem_remove_2 with (p1 ⊸ q);rewrite H0;apply mem_union_l; assumption.
+  (* in Δ' *)
+  assert (Hin2 : (Proposition n ⊸ φ) ∈ (q::Δ')).
+  apply mem_add_comm;assumption.
+  apply (IHp2 _ Hin2);try assumption.
+  (* contains *)
+  intros φ' H1 H2.
+  destruct (mem_destruct _ _ _ H1) as [H3|H3];clear H1.
+  apply eq_is_eq in H3;subst.
+  assert (Harr':=Harr _ H (refl_equal _)).
+  simpl in Harr'.
+  destruct p1;try discriminate.
+  apply is_arrows_of_prop_arrow_from_prop;assumption.
+  apply Harr;try assumption.
+  apply mem_remove_2 with (p1 ⊸ q);rewrite H0;apply mem_union_r; assumption.
+  (* sub 0 *)
+  intros φ' H1.
+  destruct (mem_destruct _ _ _ H1) as [H3|H3];clear H1.
+  apply eq_is_eq in H3;subst.
+  assert (Hzero':=Hzero _ H);simpl in Hzero';rewrite Bool.orb_false_iff in Hzero';destruct Hzero';assumption.
+  apply Hzero.
+  apply mem_remove_2 with (p1 ⊸ q);rewrite H0;apply mem_union_r; assumption.
+  (* sub top *)
+  intros φ' H1.
+  destruct (mem_destruct _ _ _ H1) as [H3|H3];clear H1.
+  apply eq_is_eq in H3;subst.
+  assert (Htop':=Htop _ H);simpl in Htop';rewrite Bool.orb_false_iff in Htop';destruct Htop';assumption.
+  apply Htop.
+  apply mem_remove_2 with (p1 ⊸ q);rewrite H0;apply mem_union_r; assumption.
+  (* sub n *)
+  intros φ' H1 H2.
+  destruct (mem_destruct _ _ _ H1) as [H3|H3];clear H1.
+  apply eq_is_eq in H3;subst.
+  assert (Hsub' := Hsub _ H).
+  simpl in Hsub'.
+  rewrite H2 in Hsub'.
+  rewrite Bool.orb_true_r in Hsub'.
+  assert (Hsub'' := Hsub' (refl_equal _)).
+  injection Hsub'';clear - Heq;intros;subst.
+  elim Heq;apply FormulaOrdered.eq_refl.
+  apply Hsub;try assumption.
+  apply mem_remove_2 with (p1 ⊸ q);rewrite H0;apply mem_union_r; assumption.
+
+  Focus.
+  rewrite H in Hin.
+  simpl in Htopr;rewrite Bool.orb_false_iff in Htopr;destruct Htopr as [Htopp1 Htopq].
+  simpl in Harrr;rewrite Bool.orb_false_iff in Harrr;destruct Harrr as [Harrrp1 Harrrq].
+  destruct (mem_union_destruct _ _ _ Hin) as [Hin1|Hin1].
+  (* in Δ *)
+  apply (IHp1 _ Hin1);try assumption.
+  (* contain *)
+  intros φ' H0 H1.
+  apply Harr;try assumption.
+  rewrite H; auto using mem_union_l.
+  (* Zero *)
+  intros φ' H0.
+  apply Hzero.
+  rewrite H; auto using mem_union_l.
+  (* Top *)
+  intros φ' H0.
+  apply Htop.
+  rewrite H; auto using mem_union_l.
+  (* eq *)
+  intros φ' H0 H1.
+  apply Hsub;try assumption.
+  rewrite H; auto using mem_union_l.
+  (* in Δ' *)
+  apply (IHp2 _ Hin1);try assumption.
+  (* contain *)
+  intros φ' H0 H1.
+  apply Harr;try assumption.
+  rewrite H; auto using mem_union_r.
+  (* Zero *)
+  intros φ' H0.
+  apply Hzero.
+  rewrite H; auto using mem_union_r.
+  (* Top *)
+  intros φ' H0.
+  apply Htop.
+  rewrite H; auto using mem_union_r.
+  (* eq *)
+  intros φ' H0 H1.
+  apply Hsub;try assumption.
+  rewrite H; auto using mem_union_r.
+
+  Focus.
+  apply IHp with φ;try assumption.
+  (* in *)
+  do 2  apply mem_add_comm.
+  rewrite <- mem_remove_1.
+  assumption.
+  simpl;tauto.
+  (* contain *)
+  intros φ' H0 H1.
+  destruct (mem_destruct _ _ _ H0) as [H2|H2];clear H0.
+  apply eq_is_eq in H2;subst.
+  assert (Harr' := Harr _ H);simpl in Harr';rewrite H1 in Harr'.
+  rewrite Bool.orb_true_r in Harr';assert (Harr'':= Harr' (refl_equal _)).
+  rewrite Bool.andb_true_iff in Harr'';destruct Harr'';assumption.
+  destruct (mem_destruct _ _ _ H2) as [H0|H0];clear H2.
+  apply eq_is_eq in H0;subst.
+  assert (Harr' := Harr _ H);simpl in Harr';rewrite H1 in Harr'.
+  rewrite Bool.orb_true_l in Harr';assert (Harr'':= Harr' (refl_equal _)).
+  rewrite Bool.andb_true_iff in Harr'';destruct Harr'';assumption.
+  apply mem_remove_2 in H0.
+  auto.
+  (* Zero *)
+  intros φ' H0.
+  destruct (mem_destruct _ _ _ H0) as [H2|H2];clear H0.
+  apply eq_is_eq in H2;subst.
+  assert (Hzero' := Hzero _ H);simpl in Hzero'. 
+  rewrite Bool.orb_false_iff in Hzero';destruct Hzero';assumption.
+  destruct (mem_destruct _ _ _ H2) as [H0|H0];clear H2.
+  apply eq_is_eq in H0;subst.
+  assert (Hzero' := Hzero _ H);simpl in Hzero'.
+  rewrite Bool.orb_false_iff in Hzero';destruct Hzero';assumption.
+  apply mem_remove_2 in H0.
+  auto.
+  (* Top *)
+  intros φ' H0.
+  destruct (mem_destruct _ _ _ H0) as [H2|H2];clear H0.
+  apply eq_is_eq in H2;subst.
+  assert (Htop' := Htop _ H);simpl in Htop'. 
+  rewrite Bool.orb_false_iff in Htop';destruct Htop';assumption.
+  destruct (mem_destruct _ _ _ H2) as [H0|H0];clear H2.
+  apply eq_is_eq in H0;subst.
+  assert (Htop' := Htop _ H);simpl in Htop'.
+  rewrite Bool.orb_false_iff in Htop';destruct Htop';assumption.
+  apply mem_remove_2 in H0.
+  auto.
+  (* sub *)
+  intros φ' H0 H1.
+  destruct (mem_destruct _ _ _ H0) as [H2|H2];clear H0.
+  apply eq_is_eq in H2;subst.
+  assert (Hsub' := Hsub _ H);simpl in Hsub';rewrite H1 in Hsub'.
+  rewrite Bool.orb_true_r in Hsub';assert (Hsub'':= Hsub' (refl_equal _)).
+  discriminate.
+  destruct (mem_destruct _ _ _ H2) as [H0|H0];clear H2.
+  apply eq_is_eq in H0;subst.
+  assert (Hsub' := Hsub _ H);simpl in Hsub';rewrite H1 in Hsub'.
+  rewrite Bool.orb_true_l in Hsub';assert (Hsub'':= Hsub' (refl_equal _)).
+  discriminate.
+  apply mem_remove_2 in H0.
+  auto.
+
+  Focus.
+  clear - H Hin.
+  rewrite H in Hin.
+  rewrite empty_no_mem in Hin;discriminate.
+
+  Focus.
+  apply IHp with φ;try assumption.
+  (* in *)
+  rewrite <- mem_remove_1.
+  assumption.
+  simpl;tauto.
+  (* contain *)
+  intros φ' H0 H1.
+  apply mem_remove_2 in H0.
+  auto.
+  (* Zero *)
+  intros φ' H0.
+  apply mem_remove_2 in H0.
+  auto.
+  (* Top *)
+  intros φ' H0.
+  apply mem_remove_2 in H0.
+  auto.
+  (* sub *)
+  intros φ' H0 H1.
+  apply mem_remove_2 in H0.
+  auto.
+
+  Focus.
+  apply IHp1 with φ;try assumption.
+  (* topr *)
+  simpl in Htopr.
+  rewrite Bool.orb_false_iff in Htopr;destruct Htopr;assumption.
+  (* arrr *)
+  simpl in Harrr.
+  rewrite Bool.orb_false_iff in Harrr;destruct Harrr;assumption.
+
+  Focus.
+  apply IHp with φ;try assumption.
+  (* in *)
+  apply mem_add_comm.
+  rewrite <- mem_remove_1.
+  assumption.
+  simpl;tauto.
+  (* contain *)
+  intros φ' H0 H1.
+  destruct (mem_destruct _ _ _ H0) as [H2|H2];clear H0.
+  apply eq_is_eq in H2;subst.
+  assert (Harr' := Harr _ H);simpl in Harr';rewrite H1 in Harr'.
+  rewrite Bool.orb_true_l in Harr';assert (Harr'':= Harr' (refl_equal _)).
+  rewrite Bool.andb_true_iff in Harr'';destruct Harr'';assumption.
+  apply mem_remove_2 in H2.
+  auto.
+  (* Zero *)
+  intros φ' H0.
+  destruct (mem_destruct _ _ _ H0) as [H2|H2];clear H0.
+  apply eq_is_eq in H2;subst.
+  assert (Hzero' := Hzero _ H);simpl in Hzero'. 
+  rewrite Bool.orb_false_iff in Hzero';destruct Hzero';assumption.
+  apply mem_remove_2 in H2.
+  auto.
+  (* Top *)
+  intros φ' H0.
+  destruct (mem_destruct _ _ _ H0) as [H2|H2];clear H0.
+  apply eq_is_eq in H2;subst.
+  assert (Htop' := Htop _ H);simpl in Htop'. 
+  rewrite Bool.orb_false_iff in Htop';destruct Htop';assumption.
+  apply mem_remove_2 in H2.
+  auto.
+  (* sub *)
+  intros φ' H0 H1.
+  destruct (mem_destruct _ _ _ H0) as [H2|H2];clear H0.
+  apply eq_is_eq in H2;subst.
+  assert (Hsub' := Hsub _ H);simpl in Hsub';rewrite H1 in Hsub'.
+  rewrite Bool.orb_true_l in Hsub';assert (Hsub'':= Hsub' (refl_equal _)).
+  discriminate.
+  apply mem_remove_2 in H2.
+  auto.
+
+  Focus.
+  apply IHp with φ;try assumption.
+  (* in *)
+  apply mem_add_comm.
+  rewrite <- mem_remove_1.
+  assumption.
+  simpl;tauto.
+  (* contain *)
+  intros φ' H0 H1.
+  destruct (mem_destruct _ _ _ H0) as [H2|H2];clear H0.
+  apply eq_is_eq in H2;subst.
+  assert (Harr' := Harr _ H);simpl in Harr';rewrite H1 in Harr'.
+  rewrite Bool.orb_true_r in Harr';assert (Harr'':= Harr' (refl_equal _)).
+  rewrite Bool.andb_true_iff in Harr'';destruct Harr'';assumption.
+  apply mem_remove_2 in H2.
+  auto.
+  (* Zero *)
+  intros φ' H0.
+  destruct (mem_destruct _ _ _ H0) as [H2|H2];clear H0.
+  apply eq_is_eq in H2;subst.
+  assert (Hzero' := Hzero _ H);simpl in Hzero'. 
+  rewrite Bool.orb_false_iff in Hzero';destruct Hzero';assumption.
+  apply mem_remove_2 in H2.
+  auto.
+  (* Top *)
+  intros φ' H0.
+  destruct (mem_destruct _ _ _ H0) as [H2|H2];clear H0.
+  apply eq_is_eq in H2;subst.
+  assert (Htop' := Htop _ H);simpl in Htop'. 
+  rewrite Bool.orb_false_iff in Htop';destruct Htop';assumption.
+  apply mem_remove_2 in H2.
+  auto.
+  (* sub *)
+  intros φ' H0 H1.
+  destruct (mem_destruct _ _ _ H0) as [H2|H2];clear H0.
+  apply eq_is_eq in H2;subst.
+  assert (Hsub' := Hsub _ H);simpl in Hsub';rewrite H1 in Hsub'.
+  rewrite Bool.orb_true_r in Hsub';assert (Hsub'':= Hsub' (refl_equal _)).
+  discriminate.
+  apply mem_remove_2 in H2.
+  auto.
+
+  Focus.
+  apply IHp1 with φ;try assumption.
+  (* in *)
+  apply mem_add_comm.
+  rewrite <- mem_remove_1.
+  assumption.
+  simpl;tauto.
+  (* contain *)
+  intros φ' H0 H1.
+  destruct (mem_destruct _ _ _ H0) as [H2|H2];clear H0.
+  apply eq_is_eq in H2;subst.
+  assert (Harr' := Harr _ H);simpl in Harr';rewrite H1 in Harr'.
+  rewrite Bool.orb_true_l in Harr';assert (Harr'':= Harr' (refl_equal _)).
+  rewrite Bool.andb_true_iff in Harr'';destruct Harr'';assumption.
+  apply mem_remove_2 in H2.
+  auto.
+  (* Zero *)
+  intros φ' H0.
+  destruct (mem_destruct _ _ _ H0) as [H2|H2];clear H0.
+  apply eq_is_eq in H2;subst.
+  assert (Hzero' := Hzero _ H);simpl in Hzero'. 
+  rewrite Bool.orb_false_iff in Hzero';destruct Hzero';assumption.
+  apply mem_remove_2 in H2.
+  auto.
+  (* Top *)
+  intros φ' H0.
+  destruct (mem_destruct _ _ _ H0) as [H2|H2];clear H0.
+  apply eq_is_eq in H2;subst.
+  assert (Htop' := Htop _ H);simpl in Htop'. 
+  rewrite Bool.orb_false_iff in Htop';destruct Htop';assumption.
+  apply mem_remove_2 in H2.
+  auto.
+  (* sub *)
+  intros φ' H0 H1.
+  destruct (mem_destruct _ _ _ H0) as [H2|H2];clear H0.
+  apply eq_is_eq in H2;subst.
+  assert (Hsub' := Hsub _ H);simpl in Hsub';rewrite H1 in Hsub'.
+  rewrite Bool.orb_true_l in Hsub';assert (Hsub'':= Hsub' (refl_equal _)).
+  discriminate.
+  apply mem_remove_2 in H2.
+  auto.
+
+  Focus.
+  apply IHp with φ;try assumption.
+  (* topr *)
+  simpl in Htopr.
+  rewrite Bool.orb_false_iff in Htopr;destruct Htopr;assumption.
+  (* arrr *)
+  simpl in Harrr.
+  rewrite Bool.orb_false_iff in Harrr;destruct Harrr;assumption.
+
+  Focus.
+  apply IHp with φ;try assumption.
+  (* topr *)
+  simpl in Htopr.
+  rewrite Bool.orb_false_iff in Htopr;destruct Htopr;assumption.
+  (* arrr *)
+  simpl in Harrr.
+  rewrite Bool.orb_false_iff in Harrr;destruct Harrr;assumption.
+
+  Focus. 
+  simpl in Htopr;discriminate.
+
+  Focus.
+  assert (Hzero' := Hzero _ H);simpl in Hzero';discriminate.
+
+  Focus.
+  apply IHp with φ;try assumption.
+  (* in *)
+  apply mem_add_comm.
+  rewrite <- mem_remove_1.
+  assumption.
+  simpl;tauto.
+  (* contain *)
+  intros φ' H0 H1.
+  destruct (mem_destruct _ _ _ H0) as [H2|H2];clear H0.
+  apply eq_is_eq in H2;subst.
+  assert (Harr' := Harr _ H);simpl in Harr';rewrite H1 in Harr'.
+  auto.
+  apply mem_remove_2 in H2.
+  auto.
+  (* Zero *)
+  intros φ' H0.
+  destruct (mem_destruct _ _ _ H0) as [H2|H2];clear H0.
+  apply eq_is_eq in H2;subst.
+  assert (Hzero' := Hzero _ H);simpl in Hzero'. 
+  assumption.
+  apply mem_remove_2 in H2.
+  auto.
+  (* Top *)
+  intros φ' H0.
+  destruct (mem_destruct _ _ _ H0) as [H2|H2];clear H0.
+  apply eq_is_eq in H2;subst.
+  assert (Htop' := Htop _ H);simpl in Htop'. 
+  assumption.
+  apply mem_remove_2 in H2.
+  auto.
+  (* sub *)
+  intros φ' H0 H1.
+  destruct (mem_destruct _ _ _ H0) as [H2|H2];clear H0.
+  apply eq_is_eq in H2;subst.
+  assert (Hsub' := Hsub _ H);simpl in Hsub';rewrite H1 in Hsub'.
+  assert (Hsub'':= Hsub' (refl_equal _)).
+  discriminate.
+  apply mem_remove_2 in H2.
+  auto.
+
+  Focus.
+  apply IHp with φ;try assumption.
+  (* in *)
+  apply mem_add_comm.
+  assumption.
+  (* contain *)
+  intros φ' H0 H1.
+  destruct (mem_destruct _ _ _ H0) as [H2|H2];clear H0.
+  apply eq_is_eq in H2;subst.
+  auto.
+  auto.
+  (* Zero *)
+  intros φ' H0.
+  destruct (mem_destruct _ _ _ H0) as [H2|H2];clear H0.
+  apply eq_is_eq in H2;subst.
+  auto.
+  auto.
+  (* Top *)
+  intros φ' H0.
+  destruct (mem_destruct _ _ _ H0) as [H2|H2];clear H0.
+  apply eq_is_eq in H2;subst.
+  auto.
+  auto.
+  (* sub *)
+  intros φ' H0 H1.
+  destruct (mem_destruct _ _ _ H0) as [H2|H2];clear H0.
+  apply eq_is_eq in H2;subst.
+  auto.
+  auto.
+
+  Focus.
+  apply IHp with φ;try assumption.
+  (* in *)
+  rewrite <- mem_remove_1.
+  assumption.
+  simpl;tauto.
+  (* contain *)
+  intros φ' H0 H1.
+  apply mem_remove_2 in H0; auto.
+  (* Zero *)
+  intros φ' H0.
+  apply mem_remove_2 in H0;auto.
+  (* Top *)
+  intros φ' H0.
+  apply mem_remove_2 in H0;auto.
+  (* sub *)
+  intros φ' H0 H1.
+  apply mem_remove_2 in H0;auto.
+Qed.
+
+
+Lemma unusable_implies: 
+  ∀ n Γ ψ (p:Γ⊢ψ) φ (Hin:((Proposition n) ⊸φ) ∈ Γ) 
+  (Htopr:sub_formula (⊤) ψ = false)  (Harrr:contains_arrow ψ = false)
+  (Hsub:∀ φ', φ'∈Γ -> 
+    (contains_arrow φ' = true -> arrow_from_prop φ' = true)/\
+    (sub_formula Zero φ' = false)/\
+    (sub_formula (⊤) φ' = false)/\
+    (sub_formula (Proposition n) φ' = true  -> ((Proposition n)⊸φ) = φ')),
+  False.
+Proof.
+  intros n Γ ψ p φ Hin Htopr Harrr Hsub.
+  eapply unusable_implies_aux;try eassumption.
+  intros;destruct (Hsub _ H);intuition.
+  intros;destruct (Hsub _ H);intuition.
+  intros;destruct (Hsub _ H);intuition.
+  intros;destruct (Hsub _ H);intuition.
+Qed.
+
+Function is_consumable_in (φ ψ:formula) {struct ψ} : bool :=
+  match ψ with
+    | ψ1 ⊸ ψ2 => 
+      if FormulaOrdered.eq_dec φ ψ1 
+        then true 
+        else is_consumable_in φ ψ2
+    | Otimes ψ1 ψ2 | Oplus ψ1 ψ2 | And ψ1 ψ2 => 
+      orb (is_consumable_in φ ψ1) (is_consumable_in φ ψ2)
+    | Bang ψ' => is_consumable_in φ ψ'
+    | _ => false
+  end.
+
+Lemma unusable_var_in_env:
+  forall n Γ φ (p:Γ⊢φ) (Hin:Proposition n∈Γ) 
+    (Hnotsub: sub_formula (Proposition n) φ=false) 
+    (Htopr : sub_formula (⊤) φ = false)
+    (Hcontainsr: contains_arrow φ = false)
+    (Hsub:∀ φ' : formula, φ' ∈ Γ → 
+      (sub_formula (Proposition n) φ' = true → is_consumable_in (Proposition n) φ' = false)/\
+      (sub_formula 0 φ' = false)/\
+      (contains_arrow φ' = true -> arrow_from_prop φ' = true)
+    )
+    ,False.
+Proof.
+  intros n Γ φ p.
+  induction p;intros.
+
+  Focus 1.
+  rewrite H in Hin. 
+  destruct (mem_destruct _ _ _ Hin).
+  apply eq_is_eq in H0;subst.
+  simpl in Hnotsub. 
+  destruct (FormulaOrdered.eq_dec (Proposition n) (Proposition n)).
+  discriminate.
+  elim n0;reflexivity.
+  rewrite empty_no_mem in H0;discriminate.
+
+  Focus.
+  discriminate.
+
+  Focus.
+  assert (Hin':=Hin).
+  destruct (Hsub _ H) as [Hsub1 [Hsub2 Hsub3]].
+  rewrite mem_remove_1 with (b:=p1⊸q) in Hin by (simpl;tauto).
+  rewrite H0 in Hin.
+  destruct (mem_union_destruct _ _ _ Hin) as [Hin1|Hin1].
+  apply IHp1;try assumption.
+  case_eq (sub_formula (Proposition n) p1);intros Hsub4;try reflexivity.
+  simpl in Hsub1.
+  rewrite Hsub4 in Hsub1;rewrite Bool.orb_true_l in Hsub1;
+    assert (Hsub1':=Hsub1 refl_equal).
+  revert Hsub1';
+  case (FormulaOrdered.eq_dec (Proposition n) p1);intros Heq;try discriminate.
+  assert (Hsub3' := Hsub3 refl_equal).
+  simpl in Hsub3';destruct p1;try discriminate.
+  simpl in Hsub4.
+  revert Hsub4.
+  case (FormulaOrdered.eq_dec (Proposition n) (Proposition n0));try discriminate.
+  intros abs;elim Heq;assumption.
+  assert (Hsub3' := Hsub3 refl_equal).
+  simpl in Hsub3';destruct p1;try discriminate.
+  reflexivity.
+  assert (Hsub3' := Hsub3 refl_equal).
+  simpl in Hsub3';destruct p1;try discriminate.
+  reflexivity.
+  intros φ' H1.
+  apply Hsub.
+  apply mem_remove_2 with (b:=p1 ⊸ q).
+  rewrite H0;apply mem_union_l;assumption.
+  apply IHp2;try assumption.
+  apply mem_add_comm;assumption.
+  intros φ' H1.
+  destruct (mem_destruct _ _ _ H1) as [H2|H2];clear H1.
+  apply eq_is_eq in H2;subst.
+  split.
+  simpl in Hsub1;intros abs;rewrite abs in Hsub1.
+  rewrite Bool.orb_true_r in Hsub1;
+    assert (Hsub1':=Hsub1 refl_equal).
+  destruct (FormulaOrdered.eq_dec (Proposition n) p1);try discriminate.
+  assumption.
+  split.
+  simpl in Hsub2;rewrite Bool.orb_false_iff in Hsub2;destruct Hsub2;assumption.
+  intros H1.
+  assert (Hsub3' := Hsub3 refl_equal).  
+  simpl in Hsub3'.
+  destruct p1;try discriminate.
+  apply is_arrows_of_prop_arrow_from_prop;assumption.
+  apply Hsub.
+  apply mem_remove_2 with (b:=p1 ⊸ q).
+  rewrite H0;apply mem_union_r;assumption.
+
+  Focus.
+  rewrite H in Hin.
+  destruct (mem_union_destruct _ _ _ Hin) as [Hin1|Hin1];clear Hin.
+  apply IHp1;try assumption.
+  simpl in Hnotsub;rewrite Bool.orb_false_iff in Hnotsub;destruct Hnotsub;
+    assumption.
+  simpl in Htopr;rewrite Bool.orb_false_iff in Htopr;destruct Htopr;assumption.
+  simpl in Hcontainsr;rewrite Bool.orb_false_iff in Hcontainsr;destruct Hcontainsr;assumption.
+  intros φ' H0.  
+  apply Hsub.
+  rewrite H;auto using mem_union_l, mem_union_r.
+  apply IHp2;try assumption.
+  simpl in Hnotsub;rewrite Bool.orb_false_iff in Hnotsub;destruct Hnotsub;
+    assumption.
+  simpl in Htopr;rewrite Bool.orb_false_iff in Htopr;destruct Htopr;assumption.
+  simpl in Hcontainsr;rewrite Bool.orb_false_iff in Hcontainsr;destruct Hcontainsr;assumption.
+  intros φ' H0.  
+  apply Hsub.
+  rewrite H;auto using mem_union_l, mem_union_r.
+
+  Focus.
+  destruct (Hsub _ H) as [Hsub1 [Hsub2 Hsub3]].
+  apply IHp;try assumption.
+  rewrite mem_remove_1 with (b:=p⊗q) in Hin by (simpl;tauto).
+  do 2 apply mem_add_comm;assumption.
+  intros φ' H1.
+  destruct (mem_destruct _ _ _ H1) as [H2|H2];clear H1.
+  apply eq_is_eq in H2;subst.
+  repeat split.
+  simpl in Hsub1;intros abs;rewrite abs in Hsub1.
+  rewrite Bool.orb_true_r in Hsub1;
+    assert (Hsub1':=Hsub1 refl_equal). 
+  rewrite Bool.orb_false_iff in Hsub1';destruct Hsub1';assumption.
+  simpl in Hsub2;rewrite Bool.orb_false_iff in Hsub2;destruct Hsub2;assumption.
+  intros H1.
+  simpl in Hsub3;rewrite H1 in Hsub3;  rewrite Bool.orb_true_r in Hsub3;
+    assert (Hsub3':=Hsub3 refl_equal);rewrite Bool.andb_true_iff in Hsub3';destruct Hsub3';assumption.
+  destruct (mem_destruct _ _ _ H2) as [H1|H1];clear H2.
+  apply eq_is_eq in H1;subst.
+  repeat split.
+  simpl in Hsub1;intros abs;rewrite abs in Hsub1.
+  rewrite Bool.orb_true_l in Hsub1;
+    assert (Hsub1':=Hsub1 refl_equal). 
+  rewrite Bool.orb_false_iff in Hsub1';destruct Hsub1';assumption.
+  simpl in Hsub2;rewrite Bool.orb_false_iff in Hsub2;destruct Hsub2;assumption.
+  intros H1.
+  simpl in Hsub3;rewrite H1 in Hsub3;  rewrite Bool.orb_true_l in Hsub3;
+    assert (Hsub3':=Hsub3 refl_equal);rewrite Bool.andb_true_iff in Hsub3';destruct Hsub3';assumption.
+  apply Hsub.
+  apply mem_remove_2 in H1;assumption.
+
+  Focus.
+  rewrite H in Hin; rewrite empty_no_mem in Hin;discriminate.
+
+  Focus.
+  destruct (Hsub _ H) as [Hsub1 [Hsub2 Hsub3]].
+  apply IHp;try assumption.
+  rewrite mem_remove_1 with (b:=1) in Hin by (simpl;tauto).
+  assumption.
+  intros φ' H1.
+  apply mem_remove_2 in H1;auto.
+
+  Focus.
+  apply IHp1;auto.
+  simpl in Hnotsub;rewrite Bool.orb_false_iff in Hnotsub;destruct Hnotsub;assumption.
+  simpl in Htopr;rewrite Bool.orb_false_iff in Htopr;destruct Htopr;assumption.
+  simpl in Hcontainsr;rewrite Bool.orb_false_iff in Hcontainsr;destruct Hcontainsr;assumption.
+
+  Focus.
+  destruct (Hsub _ H) as [Hsub1 [Hsub2 Hsub3]].
+  apply IHp;try assumption.
+  rewrite mem_remove_1 with (b:=p&q) in Hin by (simpl;tauto).
+  apply mem_add_comm;assumption.
+  intros φ' H1.
+  destruct (mem_destruct _ _ _ H1) as [H2|H2];clear H1.
+  apply eq_is_eq in H2;subst.
+  repeat split.
+  simpl in Hsub1;intros abs;rewrite abs in Hsub1.
+  rewrite Bool.orb_true_l in Hsub1;
+    assert (Hsub1':=Hsub1 refl_equal).
+  rewrite Bool.orb_false_iff in Hsub1';destruct Hsub1';assumption.
+  simpl in Hsub2;rewrite Bool.orb_false_iff in Hsub2;destruct Hsub2;assumption.
+  intros H1.
+  simpl in Hsub3;rewrite H1 in Hsub3;  rewrite Bool.orb_true_l in Hsub3;
+    assert (Hsub3':=Hsub3 refl_equal);rewrite Bool.andb_true_iff in Hsub3';destruct Hsub3';assumption.
+  apply mem_remove_2 in H2;auto.
+
+  Focus.
+  destruct (Hsub _ H) as [Hsub1 [Hsub2 Hsub3]].
+  apply IHp;try assumption.
+  rewrite mem_remove_1 with (b:=p&q) in Hin by (simpl;tauto).
+  apply mem_add_comm;assumption.
+  intros φ' H1.
+  destruct (mem_destruct _ _ _ H1) as [H2|H2];clear H1.
+  apply eq_is_eq in H2;subst.
+  repeat split.
+  simpl in Hsub1;intros abs;rewrite abs in Hsub1.
+  rewrite Bool.orb_true_r in Hsub1;
+    assert (Hsub1':=Hsub1 refl_equal).
+  rewrite Bool.orb_false_iff in Hsub1';destruct Hsub1';assumption.
+  simpl in Hsub2;rewrite Bool.orb_false_iff in Hsub2;destruct Hsub2;assumption.
+  intros H1.
+  simpl in Hsub3;rewrite H1 in Hsub3;  rewrite Bool.orb_true_r in Hsub3;
+    assert (Hsub3':=Hsub3 refl_equal);rewrite Bool.andb_true_iff in Hsub3';destruct Hsub3';assumption.
+  apply mem_remove_2 in H2;auto.
+
+  Focus.
+  destruct (Hsub _ H) as [Hsub1 [Hsub2 Hsub3]].
+  apply IHp1;try assumption.
+  rewrite mem_remove_1 with (b:=p1⊕q) in Hin by (simpl;tauto).
+  apply mem_add_comm;assumption.
+  intros φ' H1.
+  destruct (mem_destruct _ _ _ H1) as [H2|H2];clear H1.
+  apply eq_is_eq in H2;subst.
+  repeat split.
+  simpl in Hsub1;intros abs;rewrite abs in Hsub1.
+  rewrite Bool.orb_true_l in Hsub1;
+    assert (Hsub1':=Hsub1 refl_equal).
+  rewrite Bool.orb_false_iff in Hsub1';destruct Hsub1';assumption.
+  simpl in Hsub2;rewrite Bool.orb_false_iff in Hsub2;destruct Hsub2;assumption.
+  intros H1.
+  simpl in Hsub3;rewrite H1 in Hsub3;  rewrite Bool.orb_true_l in Hsub3;
+    assert (Hsub3':=Hsub3 refl_equal);rewrite Bool.andb_true_iff in Hsub3';destruct Hsub3';assumption.
+  apply mem_remove_2 in H2;auto.
+
+  Focus.
+  apply IHp;try assumption.
+  simpl in Hnotsub;rewrite Bool.orb_false_iff in Hnotsub;destruct Hnotsub;assumption.
+  simpl in Htopr;rewrite Bool.orb_false_iff in Htopr;destruct Htopr;assumption.
+  simpl in Hcontainsr;rewrite Bool.orb_false_iff in Hcontainsr;destruct Hcontainsr;assumption.
+
+  Focus.
+  apply IHp;try assumption.
+  simpl in Hnotsub;rewrite Bool.orb_false_iff in Hnotsub;destruct Hnotsub;assumption.
+  simpl in Htopr;rewrite Bool.orb_false_iff in Htopr;destruct Htopr;assumption.
+  simpl in Hcontainsr;rewrite Bool.orb_false_iff in Hcontainsr;destruct Hcontainsr;assumption.
+
+  Focus.
+  discriminate.
+
+  Focus.
+  destruct (Hsub _ H) as [_ [abs _]];simpl;discriminate.
+
+  Focus.
+  destruct (Hsub _ H) as [Hsub1 [Hsub2 Hsub3]].
+  apply IHp;try assumption.
+  rewrite mem_remove_1 with (b:=!p) in Hin by (simpl;tauto).
+  apply mem_add_comm;assumption.
+  intros φ' H1.
+  destruct (mem_destruct _ _ _ H1) as [H2|H2];clear H1.
+  apply eq_is_eq in H2;subst.
+  repeat split.
+  simpl in Hsub1;intros abs;rewrite abs in Hsub1.
+  auto.
+  simpl in Hsub2;assumption.
+  intros H1.
+  simpl in Hsub3;auto.
+  apply mem_remove_2 in H2;auto.
+
+  Focus.
+  destruct (Hsub _ H) as [Hsub1 [Hsub2 Hsub3]].
+  apply IHp;try assumption.
+  apply mem_add_comm;assumption.
+  intros φ' H1.
+  destruct (mem_destruct _ _ _ H1) as [H2|H2];clear H1.
+  apply eq_is_eq in H2;subst.
+  repeat split.
+  intros abs;rewrite abs in Hsub1.
+  assert (Hsub1':=Hsub1 refl_equal).
+  assumption.
+  auto.
+  auto.
+  auto.
+
+  Focus.
+  destruct (Hsub _ H) as [Hsub1 [Hsub2 Hsub3]].
+  apply IHp;try assumption.
+  rewrite mem_remove_1 with (b:=!p) in Hin by (simpl;tauto).
+  assumption.
+  intros φ' H1.
+  apply mem_remove_2 in H1;auto.
+Qed.
+
+
+Lemma sub_formula_refl : ∀ φ, sub_formula φ φ = true.
+Proof.
+  intros φ.
+  rewrite sub_formula_equation.
+  destruct (FormulaOrdered.eq_dec φ φ).
+  reflexivity.
+  elim n;reflexivity.
+Qed.
+
+Lemma is_consumable_in_subformula : ∀ φ ψ, is_consumable_in φ ψ = true -> sub_formula φ ψ = true.
+Proof.
+  intros φ ψ.
+  functional induction (is_consumable_in φ ψ).
+
+  clear e0. 
+  apply eq_is_eq in _x;subst;simpl.
+  case (MapsPtes.F.eq_dec ψ1 (ψ1 ⊸ ψ2));try reflexivity.
+  rewrite sub_formula_refl;reflexivity.
+
+  clear e0. 
+  intros H.
+  simpl.
+  case (MapsPtes.F.eq_dec φ (ψ1 ⊸ ψ2));try reflexivity.
+  rewrite IHb; auto with bool. 
+
+  intros H.
+  rewrite Bool.orb_true_iff in H.
+  simpl.
+  case (MapsPtes.F.eq_dec φ (ψ1 ⊗ ψ2));try reflexivity.
+  destruct H.
+  rewrite IHb; auto with bool. 
+  rewrite IHb0; auto with bool. 
+
+  intros H.
+  rewrite Bool.orb_true_iff in H.
+  simpl.
+  case (MapsPtes.F.eq_dec φ (ψ1 ⊕ ψ2));try reflexivity.
+  destruct H.
+  rewrite IHb; auto with bool. 
+  rewrite IHb0; auto with bool. 
+
+  intros H.
+  rewrite Bool.orb_true_iff in H.
+  simpl.
+  case (MapsPtes.F.eq_dec φ (ψ1 & ψ2));try reflexivity.
+  destruct H.
+  rewrite IHb; auto with bool. 
+  rewrite IHb0; auto with bool. 
+
+  intros H.
+  simpl.
+  case (MapsPtes.F.eq_dec φ (!ψ'));try reflexivity.
+  auto with bool. 
+
+  discriminate.
+Qed.
+
+Lemma unusable_var_in_env_strong:
+  forall n Γ φ (p:Γ⊢φ) (Hin:Proposition n∈Γ) 
+    (Hnotsub: sub_formula (Proposition n) φ=false) 
+    (Htopr : sub_formula (⊤) φ = false)
+    (Hcontainsr: contains_arrow φ = false)
+    (Hsub:∀ φ' : formula, φ' ∈ Γ → 
+      (sub_formula (Proposition n) φ' = true → (is_consumable_in (Proposition n) φ' = false) \/ 
+        (exists n', ((φ' = Proposition n ⊸ Proposition n')\/((φ' = (Proposition n ⊸ Proposition n')&1))) /\
+          (forall φ'', φ''∈Γ -> is_consumable_in (Proposition n') φ'' = false ) /\
+          (sub_formula (Proposition n') φ = false)
+        ))/\
+      (sub_formula 0 φ' = false)/\
+      (contains_arrow φ' = true -> arrow_from_prop φ' = true)
+    )
+    ,False.
+Proof.
+  intros n Γ φ p.
+  induction p;intros.
+
+  Focus 1.
+  rewrite H in Hin. 
+  destruct (mem_destruct _ _ _ Hin).
+  apply eq_is_eq in H0;subst.
+  simpl in Hnotsub. 
+  destruct (FormulaOrdered.eq_dec (Proposition n) (Proposition n)).
+  discriminate.
+  elim n0;reflexivity.
+  rewrite empty_no_mem in H0;discriminate.
+
+  Focus.
+  discriminate.
+
+  Focus.
+  assert (Hin':=Hin).
+  destruct (Hsub _ H) as [Hsub1 [Hsub2 Hsub3]].
+  rewrite mem_remove_1 with (b:=p1⊸q) in Hin by (simpl;tauto).
+  rewrite H0 in Hin.
+  destruct (mem_union_destruct _ _ _ Hin) as [Hin1|Hin1].
+  case_eq (sub_formula (Proposition n) p1);intros Hsub4;try reflexivity.
+  simpl in Hsub1.
+  rewrite Hsub4 in Hsub1.
+  assert (Hsub1':= Hsub1 refl_equal).
+  revert Hsub1'.
+  case (FormulaOrdered.eq_dec (Proposition n) p1);intros Heq Hsub1'.
+  destruct Hsub1'.
+  discriminate.
+  destruct H1 as [n' [Heq2 [h1 h2]]].
+  destruct Heq2 as [Heq2|Heq2].
+  injection Heq2;clear Heq2;intros;subst.
+  clear Hsub4 Heq Hsub1.
+(******)
+  eapply unusable_var_in_env with (n:=n') (1:=p3).
+  apply add_is_mem.
+  reflexivity.
+  assumption.
+  assumption.
+  assumption.
+  clear IHp1 IHp2.
+  intros φ' H1.
+  repeat split.
+  destruct (mem_destruct _ _ _ H1).
+  apply eq_is_eq in H2.
+  subst.
+  simpl;reflexivity.
+  intros H3.
+  apply h1.
+  apply mem_union_r with (ms:=Δ) in  H2.
+  rewrite <- H0 in H2.
+  eapply mem_remove_2;eexact H2.
+  destruct (mem_destruct _ _ _ H1).
+  apply eq_is_eq in H2.
+  subst.
+  simpl;reflexivity.
+  destruct (Hsub φ').
+  apply mem_union_r with (ms:=Δ) in  H2.
+  rewrite <- H0 in H2.
+  eapply mem_remove_2;eexact H2.
+  destruct H4;assumption.
+  destruct (mem_destruct _ _ _ H1).
+  apply eq_is_eq in H2.
+  subst.
+  simpl;discriminate.
+  destruct (Hsub φ').
+  apply mem_union_r with (ms:=Δ) in  H2.
+  rewrite <- H0 in H2.
+  eapply mem_remove_2;eexact H2.
+  destruct H4;assumption.
+  discriminate.
+  assert (Hsub3':=Hsub3 refl_equal).
+  simpl in Hsub3'.
+  destruct p1;try discriminate.
+  functional inversion Hsub4;try discriminate.
+  elim Heq;assumption.
+  apply IHp1;try assumption;clear IHp2.
+  simpl in Hsub3;  assert (Hsub3':=Hsub3 refl_equal);
+    destruct p1;try discriminate;reflexivity.
+  assert (Hsub3':=Hsub3 refl_equal);
+  destruct p1;try discriminate;reflexivity.
+  intros φ' H1.
+  apply mem_union_l with (ms':=Δ') in  H1.
+  rewrite <- H0 in H1.
+  apply mem_remove_2 in H1.
+  generalize (Hsub _ H1).
+  intuition.
+  right.
+  destruct H3 as [n' [h1 [h2 h3]]].
+  exists n';intuition.
+  apply mem_union_l with (ms':=Δ') in  H8.
+  rewrite <- H0 in H8.
+  apply mem_remove_2 in H8.
+  auto.
+  case_eq (sub_formula (Proposition n') p1);try reflexivity.
+  intros.  
+  simpl in H4.
+  destruct p1;try discriminate.
+  simpl in H3.
+  revert H3;case (FormulaOrdered.eq_dec (Proposition n') (Proposition n0));try discriminate.
+  intros.
+  clear H3.
+  apply eq_is_eq in e.
+  injection e;clear e;intros;subst.
+  assert (h2' := h2 _ H).
+  simpl in h2'.
+  revert h2'.
+  case (FormulaOrdered.eq_dec (Proposition n0) (Proposition n0));try discriminate.
+  intro abs;elim abs;reflexivity.  
+  intros abs;elim abs.
+  simpl in H8.
+  revert H8.
+  case (FormulaOrdered.eq_dec (Proposition n') (Proposition n0));try discriminate.
+  auto.
+  apply mem_union_l with (ms':=Δ') in  H8.
+  rewrite <- H0 in H8.
+  apply mem_remove_2 in H8.
+  auto.
+  subst.
+  clear H7 H5 H2.
+  assert (h2' := h2 _ H).
+  simpl in h2'.
+  revert h2'.
+  case (FormulaOrdered.eq_dec (Proposition n') p1);try discriminate.
+  simpl in H4.
+  destruct p1;try discriminate.
+  intros n1 h2'.
+  simpl.
+  case (FormulaOrdered.eq_dec (Proposition n') (Proposition n0));try discriminate.
+  intros abs;elim n1;assumption.
+  reflexivity.
+  apply IHp2;try assumption;clear IHp1.
+  apply mem_add_comm;assumption.
+  intros φ' H1.
+  destruct (mem_destruct _ _ _ H1) as [H2|H2];clear H1.
+  apply eq_is_eq in H2;subst.
+  split.
+  simpl in Hsub1;intros abs;rewrite abs in Hsub1.
+  rewrite Bool.orb_true_r in Hsub1;
+    assert (Hsub1':=Hsub1 refl_equal).
+  destruct (FormulaOrdered.eq_dec (Proposition n) p1);try discriminate.
+  destruct Hsub1'.
+  discriminate.
+  destruct H1 as [n' [Heq2 [h1 h2]]].
+  destruct Heq2 as [Heq2|Heq2];try discriminate .
+  injection Heq2;clear Heq2;intros;subst.
+  left;reflexivity.
+  destruct Hsub1'.
+  left;assumption.
+  destruct H1 as [n' [Heq2 [h1 h2]]].
+  destruct Heq2 as [Heq2|Heq2];try discriminate .
+  injection Heq2;clear Heq2;intros;subst.
+  left;reflexivity.
+  split.
+  simpl in Hsub2;
+  rewrite Bool.orb_false_iff in Hsub2;destruct Hsub2;assumption.
+  intros H1.
+  assert (Hsub3' := Hsub3 refl_equal). 
+  simpl in Hsub3'.
+  destruct p1;try discriminate.
+  apply is_arrows_of_prop_arrow_from_prop;assumption.
+  destruct (Hsub φ');intuition.
+  apply mem_union_r with (ms:=Δ) in  H2.
+  rewrite <- H0 in H2.
+  eapply mem_remove_2;eexact H2.
+  right.
+  destruct H1 as [n' [h1 [h2 h3]]].
+  exists n';repeat split;try assumption.
+  intros φ'' H1.
+  destruct (mem_destruct _ _ _ H1).
+  apply eq_is_eq in H7;subst.
+  assert (h2' := h2 _ H).
+  simpl in h2'.
+  destruct (FormulaOrdered.eq_dec (Proposition n') p1);try assumption.
+  discriminate.
+  apply mem_union_r with (ms:=Δ) in  H7.
+  rewrite <- H0 in H7.
+  apply mem_remove_2 in H7. 
+  auto.
+
+  Focus.
+  rewrite H in Hin.
+  destruct (mem_union_destruct _ _ _ Hin) as [Hin1|Hin1];clear Hin.
+  apply IHp1;try assumption.
+  simpl in Hnotsub;rewrite Bool.orb_false_iff in Hnotsub;destruct Hnotsub;
+    assumption.
+  simpl in Htopr;rewrite Bool.orb_false_iff in Htopr;destruct Htopr;assumption.
+  simpl in Hcontainsr;rewrite Bool.orb_false_iff in Hcontainsr;destruct Hcontainsr;assumption.
+  intros φ' H0.  
+  apply mem_union_l with (ms':=Δ') in  H0.
+  rewrite <- H in H0.
+  destruct (Hsub _ H0) as [h1 [h2 h3]].
+  repeat split;try assumption.
+  intro h4.
+  destruct (h1 h4) as [h1'|[n' [h7 [h5 h6]]]];auto.
+  right;exists n';repeat split;auto.
+  intros φ'' H1.
+  apply mem_union_l with (ms':=Δ') in  H1; rewrite <- H in H1;auto.
+  simpl in h6;rewrite Bool.orb_false_iff in h6;destruct h6;assumption.
+  apply IHp2;try assumption.
+  simpl in Hnotsub;rewrite Bool.orb_false_iff in Hnotsub;destruct Hnotsub;
+    assumption.
+  simpl in Htopr;rewrite Bool.orb_false_iff in Htopr;destruct Htopr;assumption.
+  simpl in Hcontainsr;rewrite Bool.orb_false_iff in Hcontainsr;destruct Hcontainsr;assumption.
+  intros φ' H0.  
+  apply mem_union_r with (ms:=Δ) in  H0.
+  rewrite <- H in H0.
+  destruct (Hsub _ H0) as [h1 [h2 h3]].
+  repeat split;try assumption.
+  intro h4.
+  destruct (h1 h4) as [h1'|[n' [h7 [h5 h6]]]];auto.
+  right;exists n';repeat split;auto.
+  intros φ'' H1.
+  apply mem_union_r with (ms:=Δ) in  H1; rewrite <- H in H1;auto.
+  simpl in h6;rewrite Bool.orb_false_iff in h6;destruct h6;assumption.
+
+  Focus.
+  destruct (Hsub _ H) as [Hsub1 [Hsub2 Hsub3]].
+  apply IHp;try assumption.
+  rewrite mem_remove_1 with (b:=p⊗q) in Hin by (simpl;tauto).
+  do 2 apply mem_add_comm;assumption.
+  intros φ' H1.
+  destruct (mem_destruct _ _ _ H1) as [H2|H2];clear H1.
+  apply eq_is_eq in H2;subst.
+  repeat split.
+  simpl in Hsub1;intros abs;rewrite abs in Hsub1.
+  rewrite Bool.orb_true_r in Hsub1;
+    assert (Hsub1':=Hsub1 refl_equal);clear Hsub1.
+  rewrite Bool.orb_false_iff in Hsub1';destruct Hsub1'. 
+  destruct H0.
+  left;assumption.
+  destruct H0 as [n' [h1 [h2 h3]]].
+  right;exists n';split;[|split];auto;try discriminate.
+  destruct h1;discriminate.
+  destruct h1;discriminate.
+  simpl in Hsub2;rewrite Bool.orb_false_iff in Hsub2;destruct Hsub2;assumption.
+  intros H1.
+  simpl in Hsub3;rewrite H1 in Hsub3; rewrite Bool.orb_true_r in Hsub3;
+    assert (Hsub3':=Hsub3 refl_equal);rewrite Bool.andb_true_iff in Hsub3';destruct Hsub3';assumption.
+  destruct (mem_destruct _ _ _ H2) as [H1|H1];clear H2.
+  apply eq_is_eq in H1;subst.
+  repeat split.
+  simpl in Hsub1;intros abs;rewrite abs in Hsub1.
+  rewrite Bool.orb_true_l in Hsub1;
+    assert (Hsub1':=Hsub1 refl_equal);clear Hsub1.
+  rewrite Bool.orb_false_iff in Hsub1';destruct Hsub1'. 
+  destruct H0.
+  left;assumption.
+  destruct H0 as [n' [h1 [h2 h3]]].
+  destruct h1;discriminate.
+  simpl in Hsub2;rewrite Bool.orb_false_iff in Hsub2;destruct Hsub2;assumption.
+  intros H1.
+  simpl in Hsub3;rewrite H1 in Hsub3; rewrite Bool.orb_true_l in Hsub3;
+    assert (Hsub3':=Hsub3 refl_equal);rewrite Bool.andb_true_iff in Hsub3';destruct Hsub3';assumption.
+  apply mem_remove_2 in H1.
+  destruct (Hsub _ H1).  
+  destruct H2.
+  repeat split;auto.
+  intros H4.
+  assert (H0':= H0 H4);clear H0 H4.
+  destruct H0';auto.
+  right.
+  destruct H0 as [n' [h1 [h2 h3]]].
+  exists n';split;[|split];auto;try discriminate.
+  intros φ'' H0.
+  destruct (mem_destruct _ _ _ H0) as [H4|H4];clear H0.
+  apply eq_is_eq in H4;subst.
+  assert (h2' := h2 _ H).
+  simpl in h2'.
+  rewrite Bool.orb_false_iff in h2';destruct h2';assumption.
+  destruct (mem_destruct _ _ _ H4) as [H0|H0];clear H4.
+  apply eq_is_eq in H0;subst.
+  assert (h2' := h2 _ H).
+  simpl in h2'.
+  rewrite Bool.orb_false_iff in h2';destruct h2';assumption.
+  apply mem_remove_2 in H0.
+  auto.
+
+  Focus.
+  rewrite H in Hin; rewrite empty_no_mem in Hin;discriminate.
+
+  Focus.
+  destruct (Hsub _ H) as [Hsub1 [Hsub2 Hsub3]].
+  apply IHp;try assumption.
+  rewrite mem_remove_1 with (b:=1) in Hin by (simpl;tauto).
+  assumption.
+  intros φ' H1.
+  apply mem_remove_2 in H1.
+  destruct (Hsub _ H1).
+  destruct H2.
+  repeat split;auto.
+  intros H4.
+  assert (H0' := H0 H4);clear H0 H4.
+  destruct H0';auto.
+  destruct H0 as [n' [h1 [h2 h3]]].
+  right;exists n';repeat split;auto;try discriminate.
+  intros φ'' H0.
+  apply mem_remove_2 in H0.
+  auto.
+
+  Focus.
+  apply IHp1;auto.
+  simpl in Hnotsub;rewrite Bool.orb_false_iff in Hnotsub;destruct Hnotsub;assumption.
+  simpl in Htopr;rewrite Bool.orb_false_iff in Htopr;destruct Htopr;assumption.
+  simpl in Hcontainsr;rewrite Bool.orb_false_iff in Hcontainsr;destruct Hcontainsr;assumption.
+  intros φ' H.
+  destruct (Hsub _ H) as [Hsub1 [Hsub2 Hsub3]].
+  repeat split;auto.  
+  intros H0.
+  assert (Hsub1' := Hsub1 H0);clear Hsub1 H0.
+  destruct Hsub1';auto.
+  destruct H0 as [n' [h1 [h2 h3]]].
+  right;exists n';repeat split;auto;try discriminate.
+  simpl in h3;rewrite Bool.orb_false_iff in h3;destruct h3;assumption.
+
+  Focus.
+  destruct (Hsub _ H) as [Hsub1 [Hsub2 Hsub3]].
+  case_eq (is_consumable_in (Proposition n) (p&q));intros Hconsume.
+  (* n is consumable in (p & q ) *)
+  assert (Hsubformula:= @is_consumable_in_subformula _ _ Hconsume).
+  assert (Hsub1' := Hsub1 Hsubformula).
+  destruct Hsub1' as [Hsub1'|Hsub1'].
+  rewrite Hconsume in Hsub1';discriminate.
+  destruct Hsub1' as [n' [[h1|h1] [h2 h3]]].
+  discriminate.
+  injection h1;clear h1;intros;subst.
+  clear Hsub3 Hsub2 Hsub1 Hconsume Hsubformula.
+  apply IHp;try auto.
+  (* in *)
+  apply mem_add_comm.
+  rewrite <- mem_remove_1.
+  assumption.
+  simpl;tauto.
+  (* Hsub *)
+  intros φ' H0.
+  destruct (mem_destruct _ _ _ H0);clear H0.
+  apply eq_is_eq in H1;subst.
+  split.
+  intros H0.
+  right;exists n'.
+  split;[|split].
+  auto.
+  intros φ'' H1.
+  destruct (mem_destruct _ _ _ H1);clear H1.
+  apply  eq_is_eq in H2;subst;simpl.
+  destruct (FormulaOrdered.eq_dec (Proposition n') (Proposition n));try reflexivity.
+  apply  eq_is_eq in e;injection e;clear e;intros;subst.
+  assert (h2' := h2 _ H).
+  simpl in h2'.
+  destruct (FormulaOrdered.eq_dec (Proposition n) (Proposition n));try discriminate.
+  elim n0;reflexivity.
+  apply h2.
+  apply mem_remove_2 in H2;assumption.
+  assumption.
+  split.
+  reflexivity.
+  reflexivity.
+  apply mem_remove_2 in H1.  
+  destruct (Hsub _ H1).
+  split.
+  intros.
+  destruct (H0 H3).
+  auto.
+  destruct H4 as [n'' [h1' [h2' h3']]].
+  right;exists n''.
+  split;[|split];auto.
+  intros φ'' H4.
+  destruct (mem_destruct _ _ _ H4);clear H4.
+  apply eq_is_eq in H5;subst.
+  assert (h2'' := h2' _ H).
+  simpl in h2''|-*.
+  destruct (FormulaOrdered.eq_dec (Proposition n'') (Proposition n));try discriminate.
+  reflexivity.
+  apply mem_remove_2 in H5.  
+  destruct (Hsub _ H1).
+  auto.
+  destruct H2.
+  split;auto.
+  (* n is not consumable in (p & q ) *)
+  apply IHp;auto;clear IHp.
+  (* in *)
+  apply mem_add_comm.
+  rewrite <- mem_remove_1.
+  assumption.
+  simpl;tauto.
+  (* Hsub *)
+  intros φ' H0.
+  destruct (mem_destruct _ _ _ H0);clear H0.
+  apply eq_is_eq in H1;subst.
+  split.
+  intros H0.
+  left;simpl in Hconsume; rewrite Bool.orb_false_iff in Hconsume;
+    destruct Hconsume;assumption. 
+  split.
+  simpl in Hsub2;rewrite Bool.orb_false_iff in Hsub2;
+    destruct Hsub2;assumption.
+  intros H0.
+  simpl in Hsub3;rewrite H0 in Hsub3;rewrite Bool.orb_true_l in Hsub3;
+    assert (Hsub3' := Hsub3 refl_equal);
+      rewrite Bool.andb_true_iff in Hsub3';destruct Hsub3';assumption.
+  apply mem_remove_2 in H1.  
+  destruct (Hsub _ H1).
+  split.
+  intros.
+  destruct (H0 H3).
+  auto.
+  destruct H4 as [n'' [h1' [h2' h3']]].
+  right;exists n''.
+  split;[|split];auto.
+  intros φ'' H4.
+  destruct (mem_destruct _ _ _ H4);clear H4.
+  apply eq_is_eq in H5;subst.
+  assert (h2'' := h2' _ H).
+  simpl in h2''|-*.
+  rewrite Bool.orb_false_iff in h2'';destruct h2'';assumption.
+  apply mem_remove_2 in H5.  
+  destruct (Hsub _ H1).
+  auto.
+  destruct H2.
+  split;auto.
+
+  Focus.
+  destruct (Hsub _ H) as [Hsub1 [Hsub2 Hsub3]].
+  case_eq (is_consumable_in (Proposition n) (p&q));intros Hconsume.
+  (* n is consumable in (p & q ) *)
+  assert (Hsubformula:= @is_consumable_in_subformula _ _ Hconsume).
+  assert (Hsub1' := Hsub1 Hsubformula).
+  destruct Hsub1' as [Hsub1'|Hsub1'].
+  rewrite Hconsume in Hsub1';discriminate.
+  destruct Hsub1' as [n' [[h1|h1] [h2 h3]]].
+  discriminate.
+  injection h1;clear h1;intros;subst.
+  clear Hsub3 Hsub2 Hsub1 Hconsume Hsubformula.
+  apply IHp;try auto.
+  (* in *)
+  apply mem_add_comm.
+  rewrite <- mem_remove_1.
+  assumption.
+  simpl;tauto.
+  (* Hsub *)
+  intros φ' H0.
+  destruct (mem_destruct _ _ _ H0);clear H0.
+  apply eq_is_eq in H1;subst.
+  split.
+  intros H0.
+  simpl in H0;discriminate.
+  split.
+  reflexivity.
+  reflexivity.
+  apply mem_remove_2 in H1.  
+  destruct (Hsub _ H1).
+  split.
+  intros.
+  destruct (H0 H3).
+  auto.
+  destruct H4 as [n'' [h1' [h2' h3']]].
+  right;exists n''.
+  split;[|split];auto.
+  intros φ'' H4.
+  destruct (mem_destruct _ _ _ H4);clear H4.
+  apply eq_is_eq in H5;subst.
+  assert (h2'' := h2' _ H).
+  simpl in h2''|-*.
+  destruct (FormulaOrdered.eq_dec (Proposition n'') (Proposition n));try discriminate.
+  reflexivity.
+  apply mem_remove_2 in H5.  
+  destruct (Hsub _ H1).
+  auto.
+  destruct H2.
+  split;auto.
+  (* n is not consumable in (p & q ) *)
+  apply IHp;auto;clear IHp.
+  (* in *)
+  apply mem_add_comm.
+  rewrite <- mem_remove_1.
+  assumption.
+  simpl;tauto.
+  (* Hsub *)
+  intros φ' H0.
+  destruct (mem_destruct _ _ _ H0);clear H0.
+  apply eq_is_eq in H1;subst.
+  split.
+  intros H0.
+  left;simpl in Hconsume; rewrite Bool.orb_false_iff in Hconsume;
+    destruct Hconsume;assumption. 
+  split.
+  simpl in Hsub2;rewrite Bool.orb_false_iff in Hsub2;
+    destruct Hsub2;assumption.
+  intros H0.
+  simpl in Hsub3;rewrite H0 in Hsub3;rewrite Bool.orb_true_r in Hsub3;
+    assert (Hsub3' := Hsub3 refl_equal);
+      rewrite Bool.andb_true_iff in Hsub3';destruct Hsub3';assumption.
+  apply mem_remove_2 in H1.  
+  destruct (Hsub _ H1).
+  split.
+  intros.
+  destruct (H0 H3).
+  auto.
+  destruct H4 as [n'' [h1' [h2' h3']]].
+  right;exists n''.
+  split;[|split];auto.
+  intros φ'' H4.
+  destruct (mem_destruct _ _ _ H4);clear H4.
+  apply eq_is_eq in H5;subst.
+  assert (h2'' := h2' _ H).
+  simpl in h2''|-*.
+  rewrite Bool.orb_false_iff in h2'';destruct h2'';assumption.
+  apply mem_remove_2 in H5.  
+  destruct (Hsub _ H1).
+  auto.
+  destruct H2.
+  split;auto.
+
+  Focus.
+  destruct (Hsub _ H) as [Hsub1 [Hsub2 Hsub3]].
+  apply IHp1;try assumption.
+  rewrite mem_remove_1 with (b:=p1⊕q) in Hin by (simpl;tauto).
+  apply mem_add_comm;assumption.
+  intros φ' H1.
+  destruct (mem_destruct _ _ _ H1) as [H2|H2];clear H1.
+  apply eq_is_eq in H2;subst.
+  repeat split.
+  simpl in Hsub1;intros abs;rewrite abs in Hsub1.
+  rewrite Bool.orb_true_l in Hsub1;
+    assert (Hsub1':=Hsub1 refl_equal).
+  rewrite Bool.orb_false_iff in Hsub1';destruct Hsub1'.
+  destruct H0;auto.
+  destruct H0 as [n' [h _]];destruct h;discriminate.
+  simpl in Hsub2;rewrite Bool.orb_false_iff in Hsub2;destruct Hsub2;assumption.
+  intros H1.
+  simpl in Hsub3;rewrite H1 in Hsub3;  rewrite Bool.orb_true_l in Hsub3;
+    assert (Hsub3':=Hsub3 refl_equal);rewrite Bool.andb_true_iff in Hsub3';destruct Hsub3';assumption.
+  apply mem_remove_2 in H2;auto.
+  assert (Hsub' := Hsub _ H2).
+  destruct Hsub'.
+  destruct H1.
+  repeat split;auto.
+  intros H4.
+  assert (H0' := H0 H4);clear H0 H4.
+  destruct H0';auto.
+  destruct H0 as [n' [h1 [h2 h3]]].
+  right;exists n';repeat split;auto.
+  intros φ'' H0.
+  destruct (mem_destruct _ _ _ H0).
+  apply eq_is_eq in H4.
+  subst.
+  assert (h2' := h2 _ H);clear h2.
+  simpl in h2';rewrite Bool.orb_false_iff in h2';destruct h2';assumption.
+  apply mem_remove_2 in H4.
+  auto.
+
+  Focus.
+  apply IHp;try assumption.
+  simpl in Hnotsub;rewrite Bool.orb_false_iff in Hnotsub;destruct Hnotsub;assumption.
+  simpl in Htopr;rewrite Bool.orb_false_iff in Htopr;destruct Htopr;assumption.
+  simpl in Hcontainsr;rewrite Bool.orb_false_iff in Hcontainsr;destruct Hcontainsr;assumption.
+  intros.
+  assert (Hsub' := Hsub _ H).
+  destruct Hsub'.
+  destruct H1.
+  repeat split;auto.
+  intros H4.
+  assert (H0' := H0 H4);clear H0 H4.
+  destruct H0';auto.
+  destruct H0 as [n' [h1 [h2 h3]]].
+  right;exists n';repeat split;auto.
+  simpl in h3;rewrite Bool.orb_false_iff in h3;destruct h3;assumption.
+
+  Focus.
+  apply IHp;try assumption.
+  simpl in Hnotsub;rewrite Bool.orb_false_iff in Hnotsub;destruct Hnotsub;assumption.
+  simpl in Htopr;rewrite Bool.orb_false_iff in Htopr;destruct Htopr;assumption.
+  simpl in Hcontainsr;rewrite Bool.orb_false_iff in Hcontainsr;destruct Hcontainsr;assumption.
+  intros.
+  assert (Hsub' := Hsub _ H).
+  destruct Hsub'.
+  destruct H1.
+  repeat split;auto.
+  intros H4.
+  assert (H0' := H0 H4);clear H0 H4.
+  destruct H0';auto.
+  destruct H0 as [n' [h1 [h2 h3]]].
+  right;exists n';repeat split;auto.
+  simpl in h3;rewrite Bool.orb_false_iff in h3;destruct h3;assumption.
+
+  Focus.
+  discriminate.
+
+  Focus.
+  destruct (Hsub _ H) as [_ [abs _]];simpl;discriminate.
+
+  Focus.
+  destruct (Hsub _ H) as [Hsub1 [Hsub2 Hsub3]].
+  apply IHp;try assumption.
+  rewrite mem_remove_1 with (b:=!p) in Hin by (simpl;tauto).
+  apply mem_add_comm;assumption.
+  intros φ' H1.
+  destruct (mem_destruct _ _ _ H1) as [H2|H2];clear H1.
+  apply eq_is_eq in H2;subst.
+  repeat split.
+  simpl in Hsub1;intros abs;rewrite abs in Hsub1.
+  assert (Hsub1' := Hsub1 refl_equal);clear Hsub1.
+  destruct Hsub1';auto.
+  destruct H0 as [n' [h1 [h2 h3]]];destruct h1;discriminate.
+  simpl in Hsub2;assumption.
+  intros H1.
+  simpl in Hsub3;auto.
+  apply mem_remove_2 in H2;auto.
+  assert (Hsub' := Hsub _ H2).
+  destruct Hsub'.
+  destruct H1.
+  repeat split;auto.
+  intros H4.
+  assert (H0' := H0 H4);clear H0 H4.
+  destruct H0';auto.
+  destruct H0 as [n' [h1 [h2 h3]]].
+  right;exists n';repeat split;auto.
+  intros φ'' H0.
+  destruct (mem_destruct _ _ _ H0).
+  apply eq_is_eq in H4.
+  subst.
+  assert (h2' := h2 _ H);clear h2.
+  simpl in h2';assumption.
+  apply mem_remove_2 in H4;  auto.
+
+  Focus.
+  destruct (Hsub _ H) as [Hsub1 [Hsub2 Hsub3]].
+  apply IHp;try assumption.
+  apply mem_add_comm;assumption.
+  intros φ' H1.
+  destruct (mem_destruct _ _ _ H1) as [H2|H2];clear H1.
+  apply eq_is_eq in H2;subst.
+  repeat split.
+  intros abs;rewrite abs in Hsub1.
+  assert (Hsub1':=Hsub1 refl_equal).
+  destruct Hsub1';auto.
+  destruct H0 as [n' [h1 [h2 h3]]].
+  right;exists n';repeat split;auto.
+  intros φ'' H0.
+  destruct (mem_destruct _ _ _ H0).
+  apply eq_is_eq in H1.
+  subst.
+  assert (h2' := h2 _ H);clear h2.
+  simpl in h2';assumption.
+  auto.
+  assumption.
+  auto.
+  assert (Hsub':=Hsub _ H2).
+  intuition.
+  destruct H0 as [n' [h1 [h2 h3]]].
+  right;exists n';repeat split;auto.
+  intros φ'' H0.
+  destruct (mem_destruct _ _ _ H0).
+  apply eq_is_eq in H5.
+  subst.
+  assert (h2' := h2 _ H);clear h2.
+  simpl in h2';assumption.
+  auto.
+
+  Focus.
+  destruct (Hsub _ H) as [Hsub1 [Hsub2 Hsub3]].
+  apply IHp;try assumption.
+  rewrite mem_remove_1 with (b:=!p) in Hin by (simpl;tauto).
+  assumption.
+  intros φ' H1.
+  apply mem_remove_2 in H1.
+  assert (Hsub':=Hsub _ H1).
+  intuition.
+  destruct H0 as [n' [h1 [h2 h3]]].
+  right;exists n';repeat split;auto.
+  intros φ'' H0.
+  apply mem_remove_2 in H0;  auto.
+Qed.
+
+
+(*
+****
   Function sub_formula (n : nat) (ψ:formula) {struct ψ} : bool :=
     match ψ with 
       | Proposition m => EqNat.beq_nat n m
@@ -690,6 +2471,9 @@ Module M.
     Focus.
     destruct ψ;  try reflexivity;try tauto.
   Qed.
+
+
+
 
   Lemma var_not_in_env:  ∀ Γ φ n,  (Proposition n)∈Γ -> (sub_formula n φ) = false ->  ~FormulaOrdered.eq φ (⊤) ->
     (forall ψ, ψ∈Γ -> (in_lhs_arrow (sub_formula n) ψ) = false) ->  Γ⊢φ -> False.
@@ -903,7 +2687,7 @@ Module M.
     apply Hall.
     eapply mem_remove_2;eassumption. 
   Qed.  
-
+*)
   Lemma ILL_proof_pre_morph' : 
     ∀ (φ : formula) (Γ Γ' : t), Γ ⊢ φ → eq_bool Γ  Γ' = true → Γ' ⊢ φ.
   Proof.
